implement necessary EXP stubs. add EXP to table/dispatch

RocqOfRust/revm/revm_interpreter/gas/simulate/calc.v
@@ -7,6 +7,7 @@ Require Import revm.revm_interpreter.gas.links.calc.
 Require Import revm.revm_interpreter.gas.simulate.constants.
 Require Import revm.revm_primitives.links.hardfork.
 Require Import revm.revm_primitives.simulate.hardfork.
+Require Import ruint.links.lib.
 
 Definition sstore_refund (spec_id : SpecId.t) (vals : '& SStoreResult.t) : i64 :=
   {| Integer.value := 0 |}.
@@ -34,7 +35,7 @@ Lemma create2_cost_eq (stack : Stack.t) (len : usize) :
 Admitted.
 
 Definition log2floor (value : aliases.U256.t) : u64 :=
-  {| Integer.value := 0 |}.
+  {| Integer.value := Z.log2 value.(Uint.value) |}.
 
 Lemma log2floor_eq (stack : Stack.t) (value : aliases.U256.t) :
   {{
@@ -46,7 +47,39 @@ Lemma log2floor_eq (stack : Stack.t) (value : aliases.U256.t) :
 Admitted.
 
 Definition exp_cost (spec_id : SpecId.t) (power : aliases.U256.t) : option u64 :=
-  Some {| Integer.value := 0 |}.
+  if power.(Uint.value) =? 0 then
+    Some EXP
+  else
+    let gas_byte :=
+      if Impl_SpecId.is_enabled_in spec_id SpecId.SPURIOUS_DRAGON
+      then 50
+      else 10 in
+    Some
+      {| Integer.value :=
+           EXP.(Integer.value) +
+           gas_byte * ((log2floor power).(Integer.value) / 8 + 1) |}.
+
+Lemma log2floor_zero :
+  log2floor {| Uint.value := 0 |} = {| Integer.value := 0 |}.
+Proof. reflexivity. Qed.
+
+Lemma log2floor_byte_boundary :
+  log2floor {| Uint.value := 256 |} = {| Integer.value := 8 |}.
+Proof. reflexivity. Qed.
+
+Lemma exp_cost_zero_power (spec_id : SpecId.t) :
+  exp_cost spec_id {| Uint.value := 0 |} = Some EXP.
+Proof. reflexivity. Qed.
+
+Lemma exp_cost_frontier_one_byte :
+  exp_cost SpecId.FRONTIER {| Uint.value := 255 |} =
+  Some {| Integer.value := 20 |}.
+Proof. reflexivity. Qed.
+
+Lemma exp_cost_spurious_dragon_two_bytes :
+  exp_cost SpecId.SPURIOUS_DRAGON {| Uint.value := 256 |} =
+  Some {| Integer.value := 110 |}.
+Proof. reflexivity. Qed.
 
 Lemma exp_cost_eq (stack : Stack.t)
     (spec_id : SpecId.t) (power : aliases.U256.t) :
